wand_demo/VST_lemmas.v
@@ -1,0 +1,29 @@
+Require Import VST.floyd.proofauto.
+Require Import WandDemo.wand_frame.
+Require Import WandDemo.wandQ_frame.
+
+Lemma ramify_PPQQ {A: Type} {NA: NatDed A} {SA: SepLog A} {CA: ClassicalSep A}: forall P Q,
+  P |-- P * (Q -* Q).
+Proof.
+  intros.
+  apply RAMIF_PLAIN.solve with emp.
+  + rewrite sepcon_emp; auto.
+  + rewrite emp_sepcon; auto.
+Qed.
+
+Lemma is_pointer_or_null_force_val_sem_cast_neutral: forall p,
+  is_pointer_or_null p -> force_val (sem_cast_neutral p) = p.
+Proof.
+  intros.
+  destruct p; try contradiction; reflexivity.
+Qed.
+
+Lemma modus_ponens_wand' {A}{ND: NatDed A}{SL: SepLog A}:
+  forall P Q R: A, P |-- Q -> P * (Q -* R) |-- R.
+Proof.
+  intros.
+  eapply derives_trans; [| apply modus_ponens_wand].
+  apply sepcon_derives; [| apply derives_refl].
+  auto.
+Qed.
+
